@prefix : <http://promsns.org/def/do#> .
@prefix owl: <http://www.w3.org/2002/07/owl#> .
@prefix rdf: <http://www.w3.org/1999/02/22-rdf-syntax-ns#> .
@prefix xml: <http://www.w3.org/XML/1998/namespace> .
@prefix xsd: <http://www.w3.org/2001/XMLSchema#> .
@prefix rdfs: <http://www.w3.org/2000/01/rdf-schema#> .
@prefix dcterms: <http://purl.org/dc/terms/> .
@base <http://promsns.org/def/decprov> .

<http://promsns.org/def/decprov> rdf:type owl:Ontology ;
                                  owl:versionIRI <http://promsns.org/def/decprov> ;
                                  owl:imports <http://www.w3.org/ns/prov-o> ;
                                  dcterms:creator "Nicholas Car"^^xsd:string ;
                                  owl:versionInfo "v1.0"^^xsd:string ;
                                  rdfs:label "Decision Provenance ontology (DecPROV)"^^xsd:string ;
                                  rdfs:comment """This ontology is a reduced-in-scope version of the [W3C Decisions and Decision-Making Incubator Group](https://www.w3.org/2005/Incubator/decision/)'s Decision Ontology (DO) which can be found at <https://github.com/nicholascar/decision-o>. It has been re-worked to align entirely with the W3C's [PROV ontology](https://www.w3.org/TR/prov-o/) since it is widely recognised that analysing the elements of decisions *post hoc* is an exercise in provenance.

Unlike the original DO, this ontology cannot be used for *normative* scenarios: it is only capable of recording decisions that have already been made (so-called *data-driven* use in the DO). This is because PROV, to which this ontology is completely mapped, does not have a templating system which can indicate what *should* occur in future scenarios.

This ontology introduces only one new element for decision modelling over that which was present in the DO: an Agent which allows agency in decision making to be recorded."""@en ;
                                  dcterms:created "2017-06-28"^^xsd:date ;
                                  dcterms:creator <http://orcid.org/0000-0002-8742-7730> ;
                                  rdfs:seeAlso "The GitHub repository containing addition documentation: http://github.com/nicholascar/decprov-ont/"@en ;
                                  dcterms:description """This ontology is a reduced-in-scope version of the [W3C Decisions and Decision-Making Incubator Group](https://www.w3.org/2005/Incubator/decision/)'s Decision Ontology (DO) which can be found at <https://github.com/nicholascar/decision-o>. It has been re-worked to align entirely with the W3C's [PROV ontology](https://www.w3.org/TR/prov-o/) since it is widely recognised that analysing the elements of decisions *post hoc* is an exercise in provenance.

Unlike the original DO, this ontology cannot be used for *normative* scenarios: it is only capable of recording decisions that have already been made (so-called *data-driven* use in the DO). This is because PROV, to which this ontology is completely mapped, does not have a templating system which can indicate what *should* occur in future scenarios.

This ontology introduces only one new element for decision modelling over that which was present in the DO: an Agent which allows agency in decision making to be recorded."""@en ;
                                  dcterms:modified "2017-08-21"@en .

#################################################################
#    Classes
#################################################################

###  http://promsns.org/def/decprov#Answer
:Answer rdf:type owl:Class ;
        rdfs:subClassOf <http://www.w3.org/ns/prov#Entity> ,
                        [ rdf:type owl:Restriction ;
                          owl:onProperty <http://www.w3.org/ns/prov#wasGeneratedBy> ;
                          owl:someValuesFrom :OptionSelection
                        ] ,
                        [ rdf:type owl:Restriction ;
                          owl:onProperty <http://www.w3.org/ns/prov#wasInfluencedBy> ;
                          owl:someValuesFrom :Question
                        ] ;
        owl:disjointWith :Decision ,
                         :Question ;
        rdfs:comment "A recorded answer to a Question"@en ;
        rdfs:label "Answer"@en .


###  http://promsns.org/def/decprov#Decision
:Decision rdf:type owl:Class ;
          rdfs:subClassOf <http://www.w3.org/ns/prov#Entity> ;
          rdfs:comment "The consequence of a DecisionMaking Activity: a recorded outcome"@en ;
          rdfs:label "Decision"@en .


###  http://promsns.org/def/decprov#DecisionMaking
:DecisionMaking rdf:type owl:Class ;
                rdfs:subClassOf <http://www.w3.org/ns/prov#Activity> ;
                owl:disjointWith :OptionSelection ;
                rdfs:comment "A temporal event in which decision processes are undertaken, such as initiating sub-questions for the question to be answered, consideration of options etc."@en ;
                rdfs:label "Decision Making"@en .


###  http://promsns.org/def/decprov#OptionSelection
:OptionSelection rdf:type owl:Class ;
                 rdfs:subClassOf <http://www.w3.org/ns/prov#Activity> ,
                                 [ rdf:type owl:Restriction ;
                                   owl:onProperty <http://www.w3.org/ns/prov#wasStartedBy> ;
                                   owl:someValuesFrom :Question
                                 ] ;
                 rdfs:comment """Option Selection is a process (prov:Activity) through which a decision-making Agent selects something.

At least two Option Selection Activities, possibly more, must be run in parrallel by an Agent and at least one must yield an outcome in order for a Question to be answered."""@en ;
                 rdfs:label "OptionSelection"@en ,
                            "Wyb√≥r opcji"@pl ;
                 rdfs:seeAlso :Decision_making .


###  http://promsns.org/def/decprov#Question
:Question rdf:type owl:Class ;
          rdfs:subClassOf <http://www.w3.org/ns/prov#Entity> ;
          rdfs:comment "A recorded question"@en ;
          rdfs:label "Question"@en .


###  http://promsns.org/def/do#Requirement
:Requirement rdf:type owl:Class ;
             rdfs:subClassOf <http://www.w3.org/ns/prov#Entity> ;
             rdfs:comment "Requirements require something from an OptionSelection Activity. They indicate their requirement with a set (a class) of objects. They are then satisified by the presense of an onject within that class. Multiple Requirements can be intersected to require very specific OptionSelection outcomes."@en ;
             rdfs:label "Requirement"@en .


#################################################################
#    Individuals
#################################################################

###  http://promsns.org/def/do#DecisionMaker
:DecisionMaker rdf:type owl:NamedIndividual ,
                        <http://www.w3.org/ns/prov#Role> .


###  Generated by the OWL API (version 4.2.8.20170104-2310) https://github.com/owlcs/owlapi
